Check nested tick rel-spec overlay algebra

theories/scheduler_delayed_cursor_generalization/nested_tick_transport/rel_spec_probe/Scheduler_Delayed_Cursor_General_Tick_Rel_Spec_Probe.thy
@@ -16,9 +16,9 @@ definition tick_port_overlay ::
   "32 word \<Rightarrow> 32 word \<Rightarrow>
    Scheduler_V611_Parse.globals \<Rightarrow> Scheduler_V611_Parse.globals"
 where
-  "tick_port_overlay depth mask c =
+  "tick_port_overlay depth irq_mask c =
      Scheduler_V611_Parse.globals.eal6_port_interrupts_disabled_'_update
-       (\<lambda>_. mask)
+       (\<lambda>_. irq_mask)
        (Scheduler_V611_Parse.globals.eal6_port_critical_depth_'_update
          (\<lambda>_. depth) c)"
 
@@ -27,53 +27,54 @@ definition tick_port_overlay_rel ::
    Scheduler_V611_Parse.globals \<Rightarrow>
    Scheduler_V611_Parse.globals \<Rightarrow> bool"
 where
-  "tick_port_overlay_rel depth mask c c0 \<longleftrightarrow>
-     c = tick_port_overlay depth mask c0"
+  "tick_port_overlay_rel depth irq_mask c c0 \<longleftrightarrow>
+     c = tick_port_overlay depth irq_mask c0"
 
 lemma tick_port_overlay_selectors [simp]:
   "Scheduler_V611_Parse.globals.eal6_port_critical_depth_'
-      (tick_port_overlay depth mask c) = depth"
+      (tick_port_overlay depth irq_mask c) = depth"
   "Scheduler_V611_Parse.globals.eal6_port_interrupts_disabled_'
-      (tick_port_overlay depth mask c) = mask"
+      (tick_port_overlay depth irq_mask c) = irq_mask"
   "Scheduler_V611_Parse.globals.uxSchedulerSuspended_'
-      (tick_port_overlay depth mask c) =
+      (tick_port_overlay depth irq_mask c) =
     Scheduler_V611_Parse.globals.uxSchedulerSuspended_' c"
   "Scheduler_V611_Parse.globals.uxMissedTicks_'
-      (tick_port_overlay depth mask c) =
+      (tick_port_overlay depth irq_mask c) =
     Scheduler_V611_Parse.globals.uxMissedTicks_' c"
   by (simp_all add: tick_port_overlay_def)
 
 lemma tick_port_overlay_idempotent [simp]:
-  "tick_port_overlay depth mask (tick_port_overlay d m c) =
-   tick_port_overlay depth mask c"
+  "tick_port_overlay depth irq_mask (tick_port_overlay d m c) =
+   tick_port_overlay depth irq_mask c"
   by (simp add: tick_port_overlay_def)
 
 lemma tick_port_overlay_missed_tick_update:
-  "tick_port_overlay depth mask
+  "tick_port_overlay depth irq_mask
       (Scheduler_V611_Parse.globals.uxMissedTicks_'_update f c) =
    Scheduler_V611_Parse.globals.uxMissedTicks_'_update f
-      (tick_port_overlay depth mask c)"
+      (tick_port_overlay depth irq_mask c)"
   by (simp add: tick_port_overlay_def)
 
 lemma tick_port_overlay_rel_post_state_iff:
   "rel_post_state
-      (rel_prod (=) (tick_port_overlay_rel depth mask)) X Y
+      (rel_prod (=) (tick_port_overlay_rel depth irq_mask)) X Y
    \<longleftrightarrow>
    X = map_post_state
-     (\<lambda>(r, s). (r, tick_port_overlay depth mask s)) Y"
-  by (cases X; cases Y)
-     (auto simp: rel_set_def tick_port_overlay_rel_def)
+     (\<lambda>(r, s). (r, tick_port_overlay depth irq_mask s)) Y"
+  by (cases X; cases Y;
+      force simp: rel_post_state.simps rel_set_def
+        tick_port_overlay_rel_def)
 
 lemma tick_port_overlay_rel_spec_iff_run:
   fixes p ::
     "('e::default, 'a, Scheduler_V611_Parse.globals) spec_monad"
   shows
-    "rel_spec p p (tick_port_overlay depth mask c) c
-       (rel_prod (=) (tick_port_overlay_rel depth mask))
+    "rel_spec p p (tick_port_overlay depth irq_mask c) c
+       (rel_prod (=) (tick_port_overlay_rel depth irq_mask))
      \<longleftrightarrow>
-     run p (tick_port_overlay depth mask c) =
+     run p (tick_port_overlay depth irq_mask c) =
        map_post_state
-         (\<lambda>(r, s). (r, tick_port_overlay depth mask s))
+         (\<lambda>(r, s). (r, tick_port_overlay depth irq_mask s))
          (run p c)"
   by (simp add: rel_spec_def tick_port_overlay_rel_post_state_iff)
 
@@ -81,64 +82,107 @@ definition tick_port_overlay_bisim ::
   "32 word \<Rightarrow> 32 word \<Rightarrow>
    ('e::default, 'a, Scheduler_V611_Parse.globals) spec_monad \<Rightarrow> bool"
 where
-  "tick_port_overlay_bisim depth mask p \<longleftrightarrow>
-     rel_spec_monad (tick_port_overlay_rel depth mask) (=) p p"
+  "tick_port_overlay_bisim depth irq_mask p \<longleftrightarrow>
+     rel_spec_monad (tick_port_overlay_rel depth irq_mask) (=) p p"
 
 lemma tick_port_overlay_bisim_iff_run:
-  "tick_port_overlay_bisim depth mask p
+  "tick_port_overlay_bisim depth irq_mask p
    \<longleftrightarrow>
-   (\<forall>c. run p (tick_port_overlay depth mask c) =
+   (\<forall>c. run p (tick_port_overlay depth irq_mask c) =
       map_post_state
-        (\<lambda>(r, s). (r, tick_port_overlay depth mask s))
+        (\<lambda>(r, s). (r, tick_port_overlay depth irq_mask s))
         (run p c))"
-  unfolding tick_port_overlay_bisim_def
-    rel_spec_monad_iff_rel_spec tick_port_overlay_rel_def
-  by (auto simp: tick_port_overlay_rel_spec_iff_run)
+proof (rule iffI)
+  assume bisim: "tick_port_overlay_bisim depth irq_mask p"
+  have bisim':
+    "rel_spec_monad (tick_port_overlay_rel depth irq_mask) (=) p p"
+    using bisim by (simp add: tick_port_overlay_bisim_def)
+  show
+    "\<forall>c. run p (tick_port_overlay depth irq_mask c) =
+       map_post_state
+         (\<lambda>(r, s). (r, tick_port_overlay depth irq_mask s))
+         (run p c)"
+  proof
+    fix c
+    have related:
+      "rel_spec p p (tick_port_overlay depth irq_mask c) c
+         (rel_prod (=) (tick_port_overlay_rel depth irq_mask))"
+      by (rule rel_spec_monadD[OF bisim'])
+         (simp add: tick_port_overlay_rel_def)
+    then show
+      "run p (tick_port_overlay depth irq_mask c) =
+       map_post_state
+         (\<lambda>(r, s). (r, tick_port_overlay depth irq_mask s))
+         (run p c)"
+      by (simp add: tick_port_overlay_rel_spec_iff_run)
+  qed
+next
+  assume runs:
+    "\<forall>c. run p (tick_port_overlay depth irq_mask c) =
+       map_post_state
+         (\<lambda>(r, s). (r, tick_port_overlay depth irq_mask s))
+         (run p c)"
+  show "tick_port_overlay_bisim depth irq_mask p"
+    unfolding tick_port_overlay_bisim_def
+  proof (rule rel_spec_monadI)
+    fix s t
+    assume related: "tick_port_overlay_rel depth irq_mask s t"
+    then have s:
+      "s = tick_port_overlay depth irq_mask t"
+      by (simp add: tick_port_overlay_rel_def)
+    show
+      "rel_spec p p s t
+         (rel_prod (=) (tick_port_overlay_rel depth irq_mask))"
+      using runs[rule_format, of t]
+      by (simp add: s tick_port_overlay_rel_spec_iff_run)
+  qed
+qed
 
 lemma tick_port_overlay_bisim_yield:
-  "tick_port_overlay_bisim depth mask (yield x)"
+  "tick_port_overlay_bisim depth irq_mask (yield x)"
   by (simp add: tick_port_overlay_bisim_iff_run)
 
 lemma tick_port_overlay_bisim_gets:
   assumes invariant:
-    "\<And>c. f (tick_port_overlay depth mask c) = f c"
-  shows "tick_port_overlay_bisim depth mask (gets f)"
+    "\<And>c. f (tick_port_overlay depth irq_mask c) = f c"
+  shows "tick_port_overlay_bisim depth irq_mask (gets f)"
   using invariant
   by (simp add: tick_port_overlay_bisim_iff_run)
 
 lemma tick_port_overlay_bisim_guard:
   assumes invariant:
-    "\<And>c. P (tick_port_overlay depth mask c) = P c"
-  shows "tick_port_overlay_bisim depth mask (guard P)"
+    "\<And>c. P (tick_port_overlay depth irq_mask c) = P c"
+  shows "tick_port_overlay_bisim depth irq_mask (guard P)"
   using invariant
-  by (simp add: tick_port_overlay_bisim_iff_run run_guard)
+  by (simp add: tick_port_overlay_bisim_iff_run run_guard
+      map_post_state_top)
 
 lemma tick_port_overlay_bisim_modify:
   assumes commute:
-    "\<And>c. f (tick_port_overlay depth mask c) =
-       tick_port_overlay depth mask (f c)"
-  shows "tick_port_overlay_bisim depth mask (modify f)"
+    "\<And>c. f (tick_port_overlay depth irq_mask c) =
+       tick_port_overlay depth irq_mask (f c)"
+  shows "tick_port_overlay_bisim depth irq_mask (modify f)"
   using commute
   by (simp add: tick_port_overlay_bisim_iff_run)
 
 lemma tick_port_overlay_bisim_condition:
   assumes invariant:
-      "\<And>c. P (tick_port_overlay depth mask c) = P c"
-    and left: "tick_port_overlay_bisim depth mask p"
-    and right: "tick_port_overlay_bisim depth mask q"
+      "\<And>c. P (tick_port_overlay depth irq_mask c) = P c"
+    and left: "tick_port_overlay_bisim depth irq_mask p"
+    and right: "tick_port_overlay_bisim depth irq_mask q"
   shows
-    "tick_port_overlay_bisim depth mask (condition P p q)"
+    "tick_port_overlay_bisim depth irq_mask (condition P p q)"
   using invariant left right
   by (simp add: tick_port_overlay_bisim_iff_run run_condition)
 
 lemma tick_port_overlay_bisim_bind:
   fixes p ::
     "('e::default, 'a, Scheduler_V611_Parse.globals) spec_monad"
-  assumes head: "tick_port_overlay_bisim depth mask p"
-    and tail: "\<And>x. tick_port_overlay_bisim depth mask (k x)"
-  shows "tick_port_overlay_bisim depth mask (p >>= k)"
+  assumes head: "tick_port_overlay_bisim depth irq_mask p"
+    and tail: "\<And>x. tick_port_overlay_bisim depth irq_mask (k x)"
+  shows "tick_port_overlay_bisim depth irq_mask (p >>= k)"
 proof -
-  let ?R = "tick_port_overlay_rel depth mask"
+  let ?R = "tick_port_overlay_rel depth irq_mask"
   have head':
     "rel_spec_monad ?R (rel_exception_or_result (=) (=)) p p"
     using head
@@ -160,7 +204,7 @@ proof -
 qed
 
 lemma tick_port_overlay_suspended_branch_bisim:
-  "tick_port_overlay_bisim depth mask
+  "tick_port_overlay_bisim depth irq_mask
      (modify
        (Scheduler_V611_Parse.globals.uxMissedTicks_'_update
          (\<lambda>a. a + 1)))"
@@ -175,14 +219,14 @@ text \<open>
 
 theorem vTaskIncrementTick_tick_port_overlay_bisim_from_unlocked:
   assumes unlocked:
-    "tick_port_overlay_bisim depth mask one_due_tick_unlocked_source"
+    "tick_port_overlay_bisim depth irq_mask one_due_tick_unlocked_source"
   shows
-    "rel_spec_monad (tick_port_overlay_rel depth mask) (=)
+    "rel_spec_monad (tick_port_overlay_rel depth irq_mask) (=)
        Scheduler_V611_Delay_Translation.vTaskIncrementTick'
        Scheduler_V611_Delay_Translation.vTaskIncrementTick'"
 proof -
   have whole:
-    "tick_port_overlay_bisim depth mask
+    "tick_port_overlay_bisim depth irq_mask
        Scheduler_V611_Delay_Translation.vTaskIncrementTick'"
     unfolding one_due_vTaskIncrementTick_named_outer_source
     apply (rule tick_port_overlay_bisim_condition)
@@ -197,7 +241,7 @@ qed
 text \<open>
   Exact remaining rule for the next checker lane:
 
-  @{term "tick_port_overlay_bisim depth mask
+  @{term "tick_port_overlay_bisim depth irq_mask
      one_due_tick_unlocked_source"}.
 
   It can be proved compositionally from the rules above plus corresponding
